split into files

pn.thy
@@ -1,29 +1,12 @@
 theory pn
-  imports Main
+  imports Base
 begin
 
-declare[[typedef_overloaded]]
-
-(* First, we have a finite number of players, places, 
-   and transitions 
-*)
-consts num_players :: "nat"
-consts num_places :: "nat"
+(* We have a finite number of transitions *)
 consts num_transitions :: "nat"
 
-(* Next, the domain for players is then defined as the
-   numbers 0, 1, ... num_players. Places and
-   transitions are defined similarily, but with
-   num_places and num_transitions respectively instead
-*)
-typedef players = "{ i . i \<le> num_players}"
-  apply(rule_tac x = 0 in exI)
-  by simp
-
-typedef places = "{ i . i \<le> num_places}"
-  apply(rule_tac x = 0 in exI)
-  by simp
-
+(* Transitions are defined similarily to players and 
+   places, but with num_transitions instead *)
 typedef transitions = "{ i . i \<le> num_transitions}"
   apply(rule_tac x = 0 in exI)
   by simp
@@ -72,7 +55,7 @@ definition T :: "transitions set" where "T \<equiv> (fst (snd PetriNet))"
 definition Q :: "trans_owner" where "Q \<equiv> (fst (snd (snd PetriNet)))"
 definition W :: "weights" where "W \<equiv> (snd (snd (snd PetriNet)))"
 
-(* All the enabled transitions in a given state *)
+(* All the enabled transitions in a given marking *)
 fun enabled :: "marking \<Rightarrow> (transitions set)"
   where
     "enabled m = 
@@ -81,15 +64,15 @@ fun enabled :: "marking \<Rightarrow> (transitions set)"
         ((m p) \<le> bound)
       }"
 
-fun enabled_p :: "marking \<Rightarrow> players \<Rightarrow> (transitions set)"
-  where
-    "enabled_p m p = { t . (t \<in> (enabled m)) \<and> ((Q t) = p) }"
+(* All the enabled transitions for a given player at a given marking *)
+fun enabled_p :: "marking \<Rightarrow> players \<Rightarrow> (transitions set)" where
+  "enabled_p m p = { t . (t \<in> (enabled m)) \<and> ((Q t) = p) }"
 
 (* Gives the marking resulting from firing a transition
    no matter if that transition is enabled or not
 *)
-fun resulting_marking :: "marking \<Rightarrow> transitions \<Rightarrow> marking"
-  where "resulting_marking m t = (\<lambda>p. (m p) - (W (PT p t)) + (W (TP t p)))"
+fun resulting_marking :: "marking \<Rightarrow> transitions \<Rightarrow> marking" where
+ "resulting_marking m t = (\<lambda>p. (m p) - (W (PT p t)) + (W (TP t p)))"
 
 (* The firing of a marking produces another marking*)
 fun fire :: "marking \<Rightarrow> transitions \<Rightarrow> (marking option)" where
@@ -104,5 +87,13 @@ lemma cannot_fire[simp]: "t \<notin> (enabled m) \<Longrightarrow> fire m t = No
 lemma can_fire[simp]: "t \<in> (enabled m) \<Longrightarrow> fire m t \<noteq> None"
   apply(simp)
   done
+
+lemma enabled_trans[simp]: "\<forall>t. t \<in> (enabled m) \<longrightarrow> t \<in> T"
+  apply(simp)
+  done
+
+lemma player_can_fire: "(t \<in> (enabled m) \<and> (Q t) = (Abs_players 1)) = (t \<in> (enabled_p m (Abs_players 1)))"
+  apply(induct_tac t)
+  oops
 
 end
