ATL.thy
@@ -1,40 +1,21 @@
 theory ATL
-  imports pn
+  imports Base
 begin
 
-datatype predop = Le | Leq | Eq | Neq | Ge | Geq
+(* The operators allowed in expressions *)
 datatype exprop = Plus | Minus | Mult
 
+(* The syntax of our expressions *)
 datatype Expr = Constant nat 
               | Place places 
               | Enabled players
               | Expr Expr exprop Expr
 
+(* The operators allowed in our predicates *)
+datatype predop = Le | Leq | Eq | Neq | Ge | Geq
+
+(* The syntax of our predicates *)
 datatype predicate = Boolean bool 
                    | Equation Expr predop Expr
 
-fun eval_e :: "marking \<Rightarrow> Expr \<Rightarrow> nat"
-  where
-    "eval_e _ (Constant b) = b"
-  | "eval_e m (Place b) = (m b)"
-  | "eval_e m (Enabled a) = card (enabled_p m a)"
-  | "eval_e m (Expr a Plus c) = ((eval_e m a) + (eval_e m c))"
-  | "eval_e m (Expr a Minus c) = ((eval_e m a) - (eval_e m c))"
-  | "eval_e m (Expr a Mult c) = ((eval_e m a) * (eval_e m c))"
-
-fun eval_p :: "marking \<Rightarrow> predicate \<Rightarrow> bool"
-  where 
-    "eval_p _ (Boolean a) = a"
-  | "eval_p s (Equation a Le c) = ((eval_e s a) < (eval_e s c))"
-  | "eval_p s (Equation a Leq c) = ((eval_e s a) \<le> (eval_e s c))"
-  | "eval_p s (Equation a Eq c) = ((eval_e s a) = (eval_e s c))"
-  | "eval_p s (Equation a Neq c) = ((eval_e s a) \<noteq> (eval_e s c))"
-  | "eval_p s (Equation a Ge c) = ((eval_e s a) > (eval_e s c))"
-  | "eval_p s (Equation a Geq c) = ((eval_e s a) \<ge> (eval_e s c))"
-
-
-datatype formula = Disjunction formula formula
-                 | Predicate predicate
-                 | Negation formula
-                 | Next players formula
-                 | Until players formula formula
+end
