EDG.thy
@@ -1,0 +1,5 @@
+theory EDG
+  imports ATL pn
+begin
+  
+end
